src/StateTransformerApplications.v
@@ -1,0 +1,137 @@
+Add LoadPath "./" as Monads .
+Require Import Monads.FunctorApplicativeMonad.
+Require Import Monads.StateMonad.
+Require Import Monads.ExnTransformer.
+Require Import NPeano Arith Bool String List.
+
+Definition state:= string -> nat.
+Definition eqb_string (x y : string) : bool :=
+  if string_dec x y then true else false.
+
+Definition state_update  (m : state )
+                    (x : string) (v : nat) :=
+  fun x' => if eqb_string x x' then v else m x'.
+  
+Definition newarray (n : nat) : state :=
+  (fun _ => n).
+
+Notation "'_' '!->' v" := (newarray v)
+  (at level 100, right associativity).
+
+Definition empty_st := (_ !-> 0).
+
+
+Inductive exp : Type :=
+  | ANum (n : nat)
+  | AId (x : string)             
+  | APlus (a1 a2 : exp)
+  | ADiv (a1 a2: exp)
+  | EqExp (a1 a2: exp).
+
+Coercion AId : string >-> exp.
+Coercion ANum : nat >-> exp.
+
+Declare Custom Entry com.
+Declare Scope com_scope.
+Notation "<{ e }>" := e (at level 0, e custom com at level 99) : com_scope.
+Notation "( x )" := x (in custom com, x at level 99) : com_scope.
+Notation "x" := x (in custom com at level 0, x constr at level 0) : com_scope.
+Notation "f x .. y" := (.. (f x) .. y)
+                  (in custom com at level 0, only parsing,
+                  f constr at level 0, x constr at level 9,
+                  y constr at level 9) : com_scope.
+Notation "x + y" := (APlus x y) (in custom com at level 50, left associativity).
+Notation "x / y" := (ADiv x y) (in custom com at level 50, left associativity).
+Notation "x == y" := (EqExp x y) (in custom com at level 50, left associativity).
+Open Scope com_scope.
+
+Definition X:string:="x"%string.
+Definition Y:string:="y"%string.
+Definition Z:string:="z"%string.
+
+Inductive com : Type :=
+  | CSkip 
+  | CAss (x : string) (a : exp)
+  | CSeq (c1 c2 : com)
+  | CIf (a: exp) (c1 c2 : com)
+  | CWhile (a: exp) (c: com).
+
+Notation "'skip'"  :=
+         CSkip (in custom com at level 0) : com_scope.
+Notation "x := y"  :=
+         (CAss x y)
+            (in custom com at level 0, x constr at level 0,
+             y at level 85, no associativity) : com_scope.
+Notation "x ; y" :=
+         (CSeq x y)
+           (in custom com at level 90, right associativity) : com_scope.
+Notation "'if' x 'then' y 'else' z 'end'" :=
+         (CIf x y z)
+           (in custom com at level 89, x at level 99,
+            y at level 99, z at level 99) : com_scope.
+Notation "'while' x 'd' y 'end'" :=
+         (CWhile x y)
+   (in custom com at level 89, x at level 99, y at level 99) : com_scope.
+   
+Definition exn_state:= exn_t (state_comp state).
+Definition eval_exn_state :=exn_state nat.
+Definition exec_exn_state :=exn_state unit.
+
+Definition fetch (x:string) : eval_exn_state := 
+  fun s =>  (Result (s x), s).
+Definition assign (x:string) (n:nat) : exec_exn_state := 
+  fun s => (Result tt, state_update s x n).
+  
+Fixpoint eval (a : exp) : eval_exn_state :=
+  match a with
+  | ANum n       => pure n
+  | AId x        => fetch x  
+  | <{a1 + a2}>  => n1 <- eval a1 ;; n2 <- eval a2 ;; pure (n1 + n2)
+  | <{a1 / a2}>  => n1 <- eval a1 ;; n2 <- eval a2 ;; match n2 with 
+                                                              | 0 => fun s => (Fail "Division by zero!", s)
+                                                              | _ => pure (n1 + n2) end
+  | <{a1 == a2}> => n1 <- eval a1 ;; n2 <- eval a2 ;; match (beq_nat n1 n2) with 
+                                                                          | true     => pure 0
+                                                                          | false    => pure 1
+                                                                          end end.
+ 
+Example ex:exp := <{Z==X/Y}>.
+Compute fst (eval ex (newarray 1)). 
+Compute fst (eval ex empty_st). 
+ 
+(*Fixpoint exec (c : com) (i : nat) : exec_exn_state :=
+  match i with
+  | O => pure (Fail "Finished gas before end of program! Try evaluating with more gas...")
+  | S i' =>
+    match c with
+      | <{ skip }>        => pure tt
+      | <{ x := a }>      => n <- eval a ;; match n with 
+                                                 | Result m =>  assign x n
+                                                 | Fail t  => fun s => (Fail t, s) 
+                                                 end
+      | <{c1; c2}>        => x <- exec c1 (S i') ;; match x with 
+                                                        | Fail t  => fun s => (Fail t, s)
+                                                        | Result m => y <- exec c1 (S i');; match y with 
+                                                                    | Fail t  => fun s => (Fail t, s)
+                                                                    | Result m => pure tt 
+                                                                    end 
+                                                        end 
+      | <{if a then c1 else c2 end}>  => m <- eval a ;; match m with 
+                                                            | Fail t  => fun s => (Fail t, s)
+                                                            | Result n => 
+                                                                match n with 
+                                                                  | 0 => exec c1 i'
+                                                                  | _ => exec c2 i'
+                                                                      end
+                                                             end 
+      | <{while b d c end}> => m <- eval b ;; match m with 
+                                                            | Fail t  => fun s => (Fail t, s)
+                                                            | Result n =>  match n with 
+                                                                  | 0 => exec c i'
+                                                                  | _ => pure tt
+                                                                  end 
+                                                             end 
+      end
+    end.
+  
+ *)
